research/lean_only_proto/DumbContracts/Examples.lean
@@ -8,6 +8,7 @@ import DumbContracts.Examples.UpdateMax
 import DumbContracts.Examples.UpdateMin
 import DumbContracts.Examples.NonZeroStore
 import DumbContracts.Examples.CompareAndSwap
+import DumbContracts.Examples.ClearIfEq
 import DumbContracts.Examples.InitOnce
 import DumbContracts.Examples.InitToOne
 import DumbContracts.Examples.SetIfGreater
